Trim Scompiler to just the denotational refinement

stanfrontend/Scompiler.v
@@ -29,8 +29,15 @@ Local Open Scope linking_scope.
 (** Pretty-printers (defined in Caml). *)
 Parameter print_CStan: Z -> CStan.program -> unit.
 
-Definition transf_stan_program(p: Stanlight.program): res Clight.program :=
+(* Source to source translations of Stanlight *)
+Definition transf_stanlight_program (p: Stanlight.program) : res Stanlight.program :=
   OK p
+  @@ time "Sampling" Sampling.transf_program
+  @@@ time "Reparameterization" Reparameterization.transf_program.
+
+(* Full translation of stanlight to Clight *)
+Definition transf_stan_program(p: Stanlight.program): res Clight.program :=
+  (transf_stanlight_program p)
   @@ time "Sampling" Sampling.transf_program
   @@@ time "Reparameterization" Reparameterization.transf_program
   @@@ time "Clightification" Clightification.transf_program
@@ -41,217 +48,19 @@ Definition transf_stan_program(p: Stanlight.program): res Clight.program :=
   @@ print (print_CStan 2)
   @@@ time "Backend" backend. 
 
-Definition ProbCompCert's_passes :=
-      mkpass Samplingproof.match_prog
-  ::: mkpass Reparameterizationproof.match_prog
-  ::: mkpass Clightificationproof.match_prog
-  ::: mkpass VariableAllocationproof.match_prog
-  ::: mkpass Targetproof.match_prog
-  ::: mkpass Sbackendproof.match_prog
-  ::: pass_nil _.
-
-Definition match_prog_test: Stanlight.program -> Clight.program -> Prop :=
-  pass_match (compose_passes ProbCompCert's_passes).
-
-Theorem transf_stan_program_match:
+Theorem transf_stanlight_program_denotational_preserved:
   forall p tp,
-  transf_stan_program p = OK tp ->
-  match_prog_test p tp.
+  transf_stanlight_program p = OK tp ->
+  denotational_refinement tp p.
 Proof.
   intros p tp T.
-  unfold transf_stan_program, time in T. rewrite ! compose_print_identity in T. simpl in T.
-  set (p1 :=  Sampling.transf_program p) in *. 
-  destruct (Reparameterization.transf_program p1) as [p2|e] eqn:P2; simpl in T; try discriminate.
-  destruct (Clightification.transf_program p2) as [p3|e] eqn:P3; simpl in T; try discriminate.
-  destruct (VariableAllocation.transf_program p3) as [p4|e] eqn:P4; simpl in T; try discriminate.
-  destruct (Target.transf_program p4) as [p5|e] eqn:P5; simpl in T; try discriminate.
-  destruct (Sbackend.backend p5) as [p6|e] eqn:P6; simpl in T; try discriminate.
-  unfold match_prog_test; simpl.
-  exists p1; split. eapply Samplingproof.transf_program_match; eauto.
-  exists p2; split. eapply Reparameterizationproof.transf_program_match; eauto.
-  exists p3; split. eapply Clightificationproof.transf_program_match; eauto.
-  exists p4; split. eapply VariableAllocationproof.transf_program_match; eauto.
-  exists p5; split. eapply Targetproof.transf_program_match; eauto.
-  exists p6; split. eapply Sbackendproof.transf_program_match; eauto.
-  inversion T.
-  reflexivity.
-Qed. 
-
-Lemma transf_stan_program_correct_pre:
-  forall p tp data params t,
-  match_prog_test p tp ->
-  transf_stan_program p = OK tp ->
-  forward_simulation (Ssemantics.semantics p data params t) (Clight.semantics1 tp).
-Proof.
-  intros p tp data params t M. unfold match_prog_test, pass_match in M; simpl in M.
-  Ltac DestructM_test :=
-    match goal with
-      [ H: exists p, _ /\ _ |- _ ] =>
-        let p := fresh "p" in let M := fresh "M" in let MM := fresh "MM" in
-        destruct H as (p & M & MM); clear H
-    end.
-  repeat DestructM_test. subst tp.
-
-  intros.
-  eapply compose_forward_simulations.
-    eapply Samplingproof.transf_program_correct; eassumption.
-  eapply compose_forward_simulations.
-    eapply Reparameterizationproof.transf_program_correct; try eassumption.
-  eapply compose_forward_simulations.
-    eapply Clightificationproof.transf_program_correct; eassumption.
-  eapply compose_forward_simulations.
-    eapply VariableAllocationproof.transf_program_correct; eassumption.
-  eapply compose_forward_simulations.
-    eapply Targetproof.transf_program_correct; eassumption.
-  eapply compose_forward_simulations.
-    eapply Sbackendproof.transf_program_correct; eassumption.  
-  eapply forward_simulation_identity; eauto.
-Qed.
-
-Theorem transf_stan_program_correct:
-  forall p tp data params t,
-  transf_stan_program p = OK tp ->
-  forward_simulation (Ssemantics.semantics p data params t) (Clight.semantics1 tp).
-Proof.
-  intros. 
-  eapply transf_stan_program_correct_pre; try eassumption.
-  eapply transf_stan_program_match; eassumption.
-Qed.
-
-Definition CompCert's_passes :=
-      mkpass SimplLocalsproof.match_prog
-  ::: mkpass Cshmgenproof.match_prog
-  ::: mkpass Cminorgenproof.match_prog
-  ::: mkpass Selectionproof.match_prog
-  ::: mkpass RTLgenproof.match_prog
-  ::: mkpass (match_if Compopts.optim_tailcalls Tailcallproof.match_prog)
-  ::: mkpass Inliningproof.match_prog
-  ::: mkpass Renumberproof.match_prog
-  ::: mkpass (match_if Compopts.optim_constprop Constpropproof.match_prog)
-  ::: mkpass (match_if Compopts.optim_constprop Renumberproof.match_prog)
-  ::: mkpass (match_if Compopts.optim_CSE CSEproof.match_prog)
-  ::: mkpass (match_if Compopts.optim_redundancy Deadcodeproof.match_prog)
-  ::: mkpass Unusedglobproof.match_prog
-  ::: mkpass Allocproof.match_prog
-  ::: mkpass Tunnelingproof.match_prog
-  ::: mkpass Linearizeproof.match_prog
-  ::: mkpass CleanupLabelsproof.match_prog
-  ::: mkpass (match_if Compopts.debug Debugvarproof.match_prog)
-  ::: mkpass Stackingproof.match_prog
-  ::: mkpass Asmgenproof.match_prog
-  ::: pass_nil _.
-
-Definition match_prog: Clight.program -> Asm.program -> Prop :=
-  pass_match (compose_passes CompCert's_passes).
-
-Theorem transf_clight_program_match:
-  forall p tp,
-  transf_clight_program p = OK tp ->
-  match_prog p tp.
-Proof. 
-  intros p tp T.
-  unfold transf_clight_program, time in T. rewrite ! compose_print_identity in T. simpl in T.
-  destruct (SimplLocals.transf_program p) as [p1|e] eqn:P2; simpl in T; try discriminate.
-  destruct (Cshmgen.transl_program p1) as [p2|e] eqn:P3; simpl in T; try discriminate.
-  destruct (Cminorgen.transl_program p2) as [p3|e] eqn:P4; simpl in T; try discriminate.
-  unfold transf_cminor_program, time in T. rewrite ! compose_print_identity in T. simpl in T.
-  destruct (Selection.sel_program p3) as [p4|e] eqn:P5; simpl in T; try discriminate.
-  destruct (RTLgen.transl_program p4) as [p5|e] eqn:P6; simpl in T; try discriminate.
-  unfold transf_rtl_program, time in T. rewrite ! compose_print_identity in T. simpl in T.
-  set (p6 := total_if Compopts.optim_tailcalls Tailcall.transf_program p5) in *.
-  destruct (Inlining.transf_program p6) as [p7|e] eqn:P8; simpl in T; try discriminate.
-  set (p8 := Renumber.transf_program p7) in *.
-  set (p9 := total_if Compopts.optim_constprop Constprop.transf_program p8) in *.
-  set (p10 := total_if Compopts.optim_constprop Renumber.transf_program p9) in *.
-  destruct (partial_if Compopts.optim_CSE CSE.transf_program p10) as [p11|e] eqn:P12; simpl in T; try discriminate.
-  destruct (partial_if Compopts.optim_redundancy Deadcode.transf_program p11) as [p12|e] eqn:P13; simpl in T; try discriminate.
-  destruct (Unusedglob.transform_program p12) as [p13|e] eqn:P14; simpl in T; try discriminate.
-  destruct (Allocation.transf_program p13) as [p14|e] eqn:P15; simpl in T; try discriminate.
-  set (p15 := Tunneling.tunnel_program p14) in *.
-  destruct (Linearize.transf_program p15) as [p16|e] eqn:P17; simpl in T; try discriminate.
-  set (p17 := CleanupLabels.transf_program p16) in *.
-  destruct (partial_if Compopts.debug Debugvar.transf_program p17) as [p18|e] eqn:P19; simpl in T; try discriminate.
-  destruct (Stacking.transf_program p18) as [p19|e] eqn:P20; simpl in T; try discriminate.
-  unfold match_prog; simpl.
-  exists p1; split. apply SimplLocalsproof.match_transf_program; auto.
-  exists p2; split. apply Cshmgenproof.transf_program_match; auto.
-  exists p3; split. apply Cminorgenproof.transf_program_match; auto.
-  exists p4; split. apply Selectionproof.transf_program_match; auto.
-  exists p5; split. apply RTLgenproof.transf_program_match; auto.
-  exists p6; split. apply total_if_match. apply Tailcallproof.transf_program_match.
-  exists p7; split. apply Inliningproof.transf_program_match; auto.
-  exists p8; split. apply Renumberproof.transf_program_match; auto.
-  exists p9; split. apply total_if_match. apply Constpropproof.transf_program_match.
-  exists p10; split. apply total_if_match. apply Renumberproof.transf_program_match.
-  exists p11; split. eapply partial_if_match; eauto. apply CSEproof.transf_program_match.
-  exists p12; split. eapply partial_if_match; eauto. apply Deadcodeproof.transf_program_match.
-  exists p13; split. apply Unusedglobproof.transf_program_match; auto.
-  exists p14; split. apply Allocproof.transf_program_match; auto.
-  exists p15; split. apply Tunnelingproof.transf_program_match.
-  exists p16; split. apply Linearizeproof.transf_program_match; auto.
-  exists p17; split. apply CleanupLabelsproof.transf_program_match; auto.
-  exists p18; split. eapply partial_if_match; eauto. apply Debugvarproof.transf_program_match.
-  exists p19; split. apply Stackingproof.transf_program_match; auto.
-  exists tp; split. apply Asmgenproof.transf_program_match; auto.
-  reflexivity.
-Qed. 
-
-Lemma transf_clight_program_correct:
-  forall p tp,
-  match_prog p tp ->
-  transf_clight_program p = OK tp ->
-  forward_simulation (Clight.semantics1 p) (Asm.semantics tp).
-Proof.
-  intros p tp M. unfold match_prog, pass_match in M; simpl in M.
-  Ltac DestructM :=
-    match goal with
-      [ H: exists p, _ /\ _ |- _ ] =>
-        let p := fresh "p" in let M := fresh "M" in let MM := fresh "MM" in
-        destruct H as (p & M & MM); clear H
-    end.
-  repeat DestructM. subst tp.
-
-  intros.
-  eapply compose_forward_simulations.
-    eapply SimplLocalsproof.transf_program_correct; eassumption.
-  eapply compose_forward_simulations.
-    eapply Cshmgenproof.transl_program_correct; eassumption.
-  eapply compose_forward_simulations.
-    eapply Cminorgenproof.transl_program_correct; eassumption.
-  eapply compose_forward_simulations.
-    eapply Selectionproof.transf_program_correct; eassumption.
-  eapply compose_forward_simulations.
-    eapply RTLgenproof.transf_program_correct; eassumption.
-  eapply compose_forward_simulations.
-    eapply match_if_simulation. eassumption. exact Tailcallproof.transf_program_correct.
-  eapply compose_forward_simulations.
-    eapply Inliningproof.transf_program_correct; eassumption.
-  eapply compose_forward_simulations. eapply Renumberproof.transf_program_correct; eassumption.
-  eapply compose_forward_simulations.
-    eapply match_if_simulation. eassumption. exact Constpropproof.transf_program_correct.
-  eapply compose_forward_simulations.
-    eapply match_if_simulation. eassumption. exact Renumberproof.transf_program_correct.
-  eapply compose_forward_simulations.
-    eapply match_if_simulation. eassumption. exact CSEproof.transf_program_correct.
-  eapply compose_forward_simulations.
-    eapply match_if_simulation. eassumption. exact Deadcodeproof.transf_program_correct; eassumption.
-  eapply compose_forward_simulations.
-    eapply Unusedglobproof.transf_program_correct; eassumption.
-  eapply compose_forward_simulations.
-    eapply Allocproof.transf_program_correct; eassumption.
-  eapply compose_forward_simulations.
-    eapply Tunnelingproof.transf_program_correct; eassumption.
-  eapply compose_forward_simulations.
-    eapply Linearizeproof.transf_program_correct; eassumption.
-  eapply compose_forward_simulations.
-    eapply CleanupLabelsproof.transf_program_correct; eassumption.
-  eapply compose_forward_simulations.
-    eapply match_if_simulation. eassumption. exact Debugvarproof.transf_program_correct.
-  eapply compose_forward_simulations.
-    eapply Stackingproof.transf_program_correct with (return_address_offset := Asmgenproof0.return_address_offset).
-    exact Asmgenproof.return_address_exists.
-    eassumption.
-  eapply Asmgenproof.transf_program_correct; eassumption.
+  unfold transf_stanlight_program, time in T. simpl in T.
+  destruct (Reparameterization.transf_program _) as [p2|e] eqn:P2; simpl in T; inv T.
+  eapply (denotational_refinement_trans); last first.
+  { eapply Samplingproof.denotational_preserved.
+    eapply Samplingproof.transf_program_match. }
+  { eapply Reparameterizationproof.denotational_preserved.
+    eapply Reparameterizationproof.transf_program_match; auto. }
 Qed.
 
 Definition transf_stan_program_complete(p: Stanlight.program): res Asm.program :=
@@ -260,21 +69,3 @@ Definition transf_stan_program_complete(p: Stanlight.program): res Asm.program :
   | OK p => transf_clight_program p
   | Error s => Error s
   end.
-  
-Theorem transf_stan_program_correct_complete:
-  forall p tp data params t,
-  transf_stan_program_complete p = OK tp ->
-  forward_simulation (Ssemantics.semantics p data params t) (Asm.semantics tp).
-Proof.
-  intros.
-  unfold transf_stan_program_complete in H.
-  case_eq (transf_stan_program p); intros.
-  rewrite H0 in H.   
-  apply (@compose_forward_simulations (Ssemantics.semantics p data params t)
-                                      (Clight.semantics1 p0) (Asm.semantics tp)).
-  apply transf_stan_program_correct; auto.
-  apply transf_clight_program_correct; auto.
-  apply transf_clight_program_match; auto.
-  rewrite H0 in H. 
-  discriminate. 
-Qed.
